\section{Identidades}

\subsection{Series}

$$\sum_{i=1}^{n} i^{2} = \frac{n(n+1)(2n+1)}{6}  \qquad  \sum_{i=1}^{n} i^{3} = \frac{n^{2}(n+1)^{2}}{4} = \left(\sum_{i=1}^n i\right)^2$$

$$ g_k(n) = \sum_{i=1}^n i^k = \frac{1}{k+1} \left( n^{k+1} + \sum_{j=1}^k \binom{k+1}{j+1} (-1)^{j+1} g_{k-j}(n) \right) $$

$$\sum_{i=0}^{n} ic^{i} = \frac{nc^{n+2} - (n+1)c^{n+1} + c}{(c-1)^{2}}, \quad c \neq 1$$

$$\sum_{i=0}^{\infty} ic^{i} = \frac{c}{(1-c)^{2}}, \quad |c| < 1$$

\subsection{Binomial Identities}

\bigskip

$$
\begin{array}{cc}
\binom{n}{k} = \frac{n}{k}\binom{n-1}{k-1}
&
\binom{n-1}{k} - \binom{n-1}{k-1} = \frac{n - 2k}{k} \binom{n}{k}
\\[10pt]
\binom{n}{h}\binom{n-h}{k} = \binom{n}{k}\binom{n-k}{h} &
\binom{n}{k} = \frac{n+1-k}{k} \binom{n}{k-1}
\\[10pt]
\sum_{k = 0}^n k\binom{n}{k} = n 2^{n-1} &
\sum_{k = 0}^n k^2 \binom{n}{k} = (n + n^2)2^{n-2}
\\[10pt]
\sum_{j = 0}^k\binom{m}{j} \binom{n-m}{k-j} = \binom{n}{k} &
\sum_{j = 0}^m \binom{m}{j}^2 = \binom{2m}{m}
\\[10pt]
\sum_{m = 0}^n \binom{m}{j} \binom{n-m}{k-j} = \binom{n+1}{k+1} &
\sum_{m = k}^n \binom{m}{k} = \binom{n+1}{k+1}
\\[10pt]
\sum_{r = 0}^m \binom{n+r}{r} = \binom{n+m+1}{m} &
\sum_{k=0}^{\lfloor n/2 \rfloor} \binom{n-k}{k} = \text{Fib}(n+1)
\\[10pt]
(x + y)^{n} = \sum_{k=0}^{n} \binom{n}{k} x^{n-k} y^{k} &
(1 + x)^{n} = \sum_{k=0}^{n} \binom{n}{k} x^{k}
\\[10pt]
2\sum_{i = L}^R \binom{n}{i} - \binom{n}{L} - \binom{n}{R} = \sum_{i = L+1}^R \binom{n+1}{i}
\end{array}
$$
